New version of go_lower, that is intended to   (1) be slightly more efficient   (2) allow a pathway to even more efficiency in the future   (3) allow better control over which "user" terms are simplified   (4) take better advantage of fully canonical forms   (5) introduce better names for variables and hypotheses;       the old "name" tactic should soon become obsolete.
The new go_lower requires that the proof goal be of the form
  ENTAIL ?Delta, ?PQR |-- ?PQR'
which is notation for   local (tc_environ Delta) && PQR |-- PQR'
Also, the LOCALS part of PQR must be a fully concrete list
of localdefs.  When you are proving a generic lemma where
the LOCALs part is just "Q" or (temp i v :: Q), use old_go_lower.

The new go_lower is incompatible in two ways:
  (1) Some variables and hypotheses will have different names.
  (2) Proof goals that are old-style entailments
      (PROP(...)LOCAL(...)SEP(...)|--_)
      are rejected, because no (tc_environ Delta) is present.

Everything in progs/ and sha/ is fixed up.

Hints for adjusting your code:
Avoid tactics that introduce old-style entailments; that is,
use semax_pre instead of semax_pre0,
use semax_post_flipped instead of semax_post_flipped',
don't make that extra call to (apply andp_left2), etc.

You can get the old behavior of go_lower by calling old_go_lower; and the old
behavior of entailer! by calling (old_go_lower; entailer!).

floyd/client_lemmas.v
@@ -968,11 +968,68 @@ Arguments ret_type !Delta /.
 
 Arguments Datatypes.id {A} x / .
 
+Inductive LLRR : Type :=
+  | LLLL : LLRR
+  | RRRR : LLRR.
+
+Definition tc_LR_strong {cs: compspecs} Delta e lr :=
+  match lr with
+  | LLLL => tc_lvalue Delta e
+  | RRRR => tc_expr Delta e
+  end.
+
+Definition tc_LR {cs: compspecs} Delta e lr :=
+  match e with
+  | Ederef e0 t =>
+     match lr with
+     | LLLL => denote_tc_assert
+                 (tc_andp 
+                   (typecheck_expr Delta e0) 
+                   (tc_bool (is_pointer_type (typeof e0))(op_result_type e)))
+     | RRRR => denote_tc_assert
+                match access_mode t with
+                | By_reference =>
+                   (tc_andp 
+                      (typecheck_expr Delta e0) 
+                      (tc_bool (is_pointer_type (typeof e0))(op_result_type e)))
+                | _ => tc_FF (deref_byvalue t)
+                end
+    end
+  | _ => tc_LR_strong Delta e lr
+  end.
+
+Definition eval_LR {cs: compspecs} e lr :=
+  match lr with
+  | LLLL => eval_lvalue e
+  | RRRR => eval_expr e
+  end.
+
+Lemma tc_LR_tc_LR_strong: forall {cs: compspecs} Delta e lr rho,
+  tc_LR Delta e lr rho && !! isptr (eval_LR e lr rho) |-- tc_LR_strong Delta e lr rho.
+Proof.
+  intros.
+  unfold tc_LR, tc_LR_strong.
+  destruct e; try solve [apply andp_left1; auto].
+  unfold tc_lvalue, tc_expr.
+  destruct lr; simpl.
+  + rewrite !denote_tc_assert_andp.
+    simpl.
+    unfold denote_tc_isptr.
+    unfold_lift.
+    auto.
+  + destruct (access_mode t); try solve [apply andp_left1; auto].
+    rewrite !denote_tc_assert_andp.
+    simpl.
+    unfold denote_tc_isptr.
+    unfold_lift.
+    auto.
+Qed.
+
 Ltac unfold_for_go_lower :=
   cbv delta [PROPx LOCALx SEPx locald_denote
                        eval_exprlist eval_expr eval_lvalue cast_expropt 
                        sem_cast eval_binop eval_unop force_val1 force_val2
-                      tc_expropt tc_expr tc_exprlist tc_lvalue 
+                      tc_expropt tc_expr tc_exprlist tc_lvalue tc_LR tc_LR_strong
                       typecheck_expr typecheck_exprlist typecheck_lvalue
                       function_body_ret_assert frame_ret_assert
                       make_args' bind_ret get_result1 retval
@@ -1001,7 +1058,7 @@ intros ?rho;
  try (simple apply grab_tc_environ; intro);
  repeat (progress unfold_for_go_lower; simpl).
 
-Ltac go_lower :=
+Ltac old_go_lower :=
  go_lower0;
  autorewrite with go_lower;
  try findvars;
@@ -1012,6 +1069,314 @@ Ltac go_lower :=
 Hint Rewrite eval_id_same : go_lower.
 Hint Rewrite eval_id_other using solve [clear; intro Hx; inversion Hx] : go_lower.
 (*Hint Rewrite Vint_inj' : go_lower.*)
+
+(*** New go_lower stuff ****)
+
+
+Lemma lower_one_temp:
+ forall t rho Delta P i v Q R S,
+  (temp_types Delta) ! i = Some (t,true) ->
+  (tc_val t v -> eval_id i rho = v ->
+   (local (tc_environ Delta) && PROPx P (LOCALx Q (SEPx R))) rho |-- S rho) ->
+  (local (tc_environ Delta) && PROPx P (LOCALx (temp i v :: Q) (SEPx R))) rho |-- S rho.
+Proof.
+intros.
+rewrite <- insert_local.
+forget (PROPx P (LOCALx Q (SEPx R))) as PQR.
+unfold local,lift1 in *.
+simpl in *. unfold_lift.
+normalize.
+rewrite prop_true_andp in H0 by auto.
+apply H0; auto.
+apply tc_eval_id_i with Delta; auto.
+Qed.
+
+Lemma lower_one_temp_Vint:
+ forall t rho Delta P i v Q R S,
+  (temp_types Delta) ! i = Some (t,true) ->
+  (tc_val t (Vint v) -> eval_id i rho = Vint v ->
+   (local (tc_environ Delta) && PROPx P (LOCALx Q (SEPx R))) rho |-- S rho) ->
+  (local (tc_environ Delta) && PROPx P (LOCALx (temp i (Vint v) :: Q) (SEPx R))) rho |-- S rho.
+Proof.
+intros.
+eapply lower_one_temp; eauto.
+Qed.
+
+Lemma lower_one_lvar:
+ forall t rho Delta P i v Q R S,
+  (isptr v -> lvar_denote i t v rho ->
+   (local (tc_environ Delta) && PROPx P (LOCALx Q (SEPx R))) rho |-- S rho) ->
+  (local (tc_environ Delta) && PROPx P (LOCALx (lvar i t v :: Q) (SEPx R))) rho |-- S rho.
+Proof.
+intros.
+rewrite <- insert_local.
+forget (PROPx P (LOCALx Q (SEPx R))) as PQR.
+unfold local,lift1 in *.
+simpl in *. unfold_lift.
+normalize.
+rewrite prop_true_andp in H by auto.
+apply H; auto.
+hnf in H1.
+destruct (Map.get (ve_of rho) i); try contradiction.
+destruct p. destruct H1; subst. apply I.
+Qed.
+
+Lemma gvar_size_compatible:
+  forall {cs: compspecs} i s rho t, 
+    gvar_denote i s rho -> 
+    sizeof cenv_cs t <= Int.modulus ->
+    size_compatible t s.
+Proof.
+intros.
+hnf in H. destruct (Map.get (ve_of rho) i) as [[? ? ] | ]; try contradiction.
+destruct (ge_of rho i); try contradiction.
+subst s.
+simpl; auto.
+Qed.
+
+Lemma gvar_align_compatible:
+  forall  {cs: compspecs} i s rho t, 
+    gvar_denote i s rho -> 
+    align_compatible t s.
+Proof.
+intros.
+hnf in H. destruct (Map.get (ve_of rho) i) as [[? ? ] | ]; try contradiction.
+destruct (ge_of rho i); try contradiction.
+subst s.
+simpl; auto.
+exists 0. reflexivity.
+Qed.
+
+Lemma sgvar_size_compatible:
+  forall {cs: compspecs} i s rho t, 
+    sgvar_denote i s rho -> 
+    sizeof cenv_cs t <= Int.modulus ->
+    size_compatible t s.
+Proof.
+intros.
+hnf in H.
+destruct (ge_of rho i); try contradiction.
+subst s.
+simpl; auto.
+Qed.
+
+Lemma sgvar_align_compatible:
+  forall  {cs: compspecs} i s rho t, 
+    sgvar_denote i s rho -> 
+    align_compatible t s.
+Proof.
+intros.
+hnf in H. 
+destruct (ge_of rho i); try contradiction.
+subst s.
+simpl; auto.
+exists 0. reflexivity.
+Qed.
+
+Lemma finish_compute_le:  Lt = Gt -> False.
+Proof. congruence. Qed.
+
+Lemma lower_one_gvar:
+ forall t {cs: compspecs} rho Delta P i v Q R S,
+  (glob_types Delta) ! i = Some t ->
+  sizeof cenv_cs t <= Int.modulus  ->
+  (isptr v -> gvar_denote i v rho ->
+     size_compatible t v -> align_compatible t v ->
+   (local (tc_environ Delta) && PROPx P (LOCALx Q (SEPx R))) rho |-- S rho) ->
+  (local (tc_environ Delta) && PROPx P (LOCALx (gvar i v :: Q) (SEPx R))) rho |-- S rho.
+Proof.
+intros.
+rewrite <- insert_local.
+forget (PROPx P (LOCALx Q (SEPx R))) as PQR.
+unfold local,lift1 in *.
+simpl in *. unfold_lift.
+normalize.
+rewrite prop_true_andp in H1 by auto.
+apply H1; auto.
+hnf in H3; destruct (Map.get (ve_of rho) i) as [[? ?] |  ]; try contradiction.
+destruct (ge_of rho i); try contradiction.
+subst. apply I.
+eapply gvar_size_compatible; eauto.
+eapply gvar_align_compatible; eauto.
+Qed.
+
+Lemma lower_one_sgvar:
+ forall t {cs: compspecs}  rho Delta P i v Q R S,
+  (glob_types Delta) ! i = Some t ->
+  sizeof cenv_cs t <= Int.modulus  ->
+  (isptr v -> sgvar_denote i v rho ->
+     size_compatible t v -> align_compatible t v ->
+   (local (tc_environ Delta) && PROPx P (LOCALx Q (SEPx R))) rho |-- S rho) ->
+  (local (tc_environ Delta) && PROPx P (LOCALx (sgvar i v :: Q) (SEPx R))) rho |-- S rho.
+Proof.
+intros.
+rewrite <- insert_local.
+forget (PROPx P (LOCALx Q (SEPx R))) as PQR.
+unfold local,lift1 in *.
+simpl in *. unfold_lift.
+normalize.
+rewrite prop_true_andp in H1 by auto.
+apply H1; auto.
+hnf in H3.
+destruct (ge_of rho i); try contradiction.
+subst. apply I.
+eapply sgvar_size_compatible; eauto.
+eapply sgvar_align_compatible; eauto.
+Qed.
+
+Lemma lower_one_prop:
+ forall  rho Delta P (P1: Prop) Q R S,
+  (P1 ->
+   (local (tc_environ Delta) && PROPx P (LOCALx Q (SEPx R))) rho |-- S rho) ->
+  (local (tc_environ Delta) && PROPx P (LOCALx (localprop P1 :: Q) (SEPx R))) rho |-- S rho.
+Proof.
+intros.
+rewrite <- insert_local.
+forget (PROPx P (LOCALx Q (SEPx R))) as PQR.
+unfold local,lift1 in *.
+simpl in *.
+normalize.
+rewrite prop_true_andp in H by auto.
+hnf in H1.
+apply H; auto.
+Qed.
+
+Lemma finish_lower:
+  forall rho D R S,
+  fold_right sepcon emp R |-- S rho ->
+  (local D && PROP() LOCAL() (SEPx R)) rho |-- S rho.
+Proof.
+intros.
+simpl.
+apply andp_left2.
+unfold_for_go_lower; simpl. normalize.
+Qed.
+
+Lemma lower_one_temp_Vint':
+ forall sz sg rho Delta P i v Q R S,
+  (temp_types Delta) ! i = Some (Tint sz sg noattr, true) ->
+  ((exists j, v = Vint j /\ tc_val (Tint sz sg noattr) (Vint j) /\ eval_id i rho = (Vint j)) ->
+   (local (tc_environ Delta) && PROPx P (LOCALx Q (SEPx R))) rho |-- S rho) ->
+  (local (tc_environ Delta) && PROPx P (LOCALx (temp i v :: Q) (SEPx R))) rho |-- S rho.
+Proof.
+intros.
+eapply lower_one_temp; eauto.
+intros.
+apply H0; auto.
+generalize H1; intro.
+hnf in H3. destruct v; try contradiction.
+exists i0. split3; auto.
+Qed.
+
+Ltac lower_one_temp_Vint' :=
+ match goal with
+ | a : name ?i |- (local _ && PROPx _ (LOCALx (temp ?i ?v :: _) _)) _ |-- _ =>
+     simple eapply lower_one_temp_Vint';
+     [ reflexivity | ];
+     let tc := fresh "TC" in 
+     clear a; intros [a [? [tc ?EVAL]]]; unfold tc_val in tc; try subst v;
+     revert tc; fancy_intro true
+ | |- (local _ && PROPx _ (LOCALx (temp _ ?v :: _) _)) _ |-- _ =>
+    is_var v;
+     simple eapply lower_one_temp_Vint';
+     [ reflexivity | ];
+    let v' := fresh "v" in rename v into v';
+     let tc := fresh "TC" in 
+     intros [v [? [tc ?EVAL]]]; unfold tc_val in tc; subst v';
+     revert tc; fancy_intro true
+ end.
+
+Lemma eq_True:
+   forall (A: Prop), A -> (A=True).
+Proof.
+intros.
+apply prop_ext; intuition.
+Qed.
+
+Ltac fold_types := 
+ fold noattr tuint tint tschar tuchar;
+ repeat match goal with
+ | |- context [Tpointer ?t noattr] => 
+      change (Tpointer t noattr) with (tptr t)
+ | |- context [Tarray ?t ?n noattr] => 
+      change (Tarray t n noattr) with (tarray t n)
+ end.
+
+Ltac fold_types1 := 
+  match goal with |- _ -> ?A =>
+  let a := fresh "H" in set (a:=A); fold_types; subst a
+  end.
+
+Ltac fold_types4 := 
+  match goal with |- _ -> _ -> _ -> _ -> ?A =>
+  let a := fresh "H" in set (a:=A); fold_types; subst a
+  end.
+
+Lemma derives_extract_PROP : 
+  forall (P1: Prop) A P QR S, 
+     (P1 -> A && PROPx P QR |-- S) ->
+     A && PROPx (P1::P) QR |-- S.
+Proof.
+unfold PROPx in *.
+intros.
+rewrite fold_right_cons.
+normalize.
+eapply derives_trans; [ | apply H; auto].
+normalize.
+Qed.
+
+Lemma ENTAIL_normal_ret_assert:
+  forall Delta P Q ek vl,
+ (ek = EK_normal -> vl = None -> ENTAIL Delta, P |-- Q) ->
+ ENTAIL Delta, normal_ret_assert P ek vl |-- normal_ret_assert Q ek vl.
+Proof.
+intros.
+unfold normal_ret_assert. normalize.
+Qed.
+
+Ltac go_lower :=
+intros;
+match goal with
+ | |- ENTAIL ?D, normal_ret_assert _ _ _ |-- _ =>
+       apply ENTAIL_normal_ret_assert; fancy_intros true
+ | |- local _ && _ |-- _ => idtac
+ | |- ENTAIL _, _ |-- _ => idtac
+ | _ => fail 10 "go_lower requires a proof goal in the form of (ENTAIL _ , _ |-- _)"
+end;
+repeat (simple apply derives_extract_PROP; fancy_intro true);
+let rho := fresh "rho" in 
+intro rho;
+repeat first
+ [ simple eapply lower_one_temp_Vint;
+     [try reflexivity; eauto | unfold tc_val at 1; fancy_intro true; intros ?EVAL ]
+ | lower_one_temp_Vint'
+ | simple eapply lower_one_temp; 
+     [try reflexivity; eauto | unfold tc_val at 1; fancy_intro true; intros ?EVAL]
+ | simple apply lower_one_lvar;
+     fold_types1; fancy_intro true; intros ?LV
+ | simple eapply lower_one_gvar;
+     [try reflexivity; eauto  | compute; apply finish_compute_le
+     | fold_types4; fancy_intro true; intros ?GV ?SC ?AC]
+ | simple eapply lower_one_sgvar;
+     [try reflexivity; eauto  | compute; apply finish_compute_le
+     | fold_types4; fancy_intro true; intros ?GV ?SC ?AC]
+ ];
+apply finish_lower;
+unfold_for_go_lower;
+simpl; rewrite ?sepcon_emp;
+repeat match goal with H: eval_id ?i rho = _ |- _ =>
+  let x := fresh "x" in 
+    set (x := eval_id i rho) in *; clearbody x; subst x
+end;
+repeat match goal with
+ | H: lvar_denote ?i ?t ?v rho |- context [lvar_denote ?i ?t' ?v' rho] =>
+     rewrite (eq_True (lvar_denote i t' v' rho) H)
+ | H: gvar_denote ?i ?v rho |- context [gvar_denote ?i ?v' rho] =>
+     rewrite (eq_True (gvar_denote i v' rho) H)
+ | H: sgvar_denote ?i ?v rho |- context [sgvar_denote ?i ?v' rho] =>
+     rewrite (eq_True (sgvar_denote i v' rho) H)
+end;
+try clear dependent rho.
 
 Lemma raise_sepcon:
  forall A B : environ -> mpred , 
@@ -1967,19 +2332,6 @@ Ltac move_from_SEP' PQR :=
       unfold replace_nth at 1
    end
  end.
-
-Lemma derives_extract_PROP : 
-  forall (P1: Prop) A P QR S, 
-     (P1 -> A && PROPx P QR |-- S) ->
-     A && PROPx (P1::P) QR |-- S.
-Proof.
-unfold PROPx in *.
-intros.
-rewrite fold_right_cons.
-normalize.
-eapply derives_trans; [ | apply H; auto].
-normalize.
-Qed.
 
 Lemma derives_extract_PROP' : 
   forall (P1: Prop) P QR S, 
