floyd/freezer.v
@@ -46,9 +46,9 @@ Lemma freeze1_SEP':
  @semax cs Espec Delta (PROPx P (LOCALx Q (SEPx R))) c Post.
 Proof.
 intros. subst.
-eapply semax_pre_post. 3: eassumption. 2: intros; entailer.
+eapply semax_pre_post. 3: eassumption. 2: intros; apply andp_left2; auto.
 apply andp_left2.
-entailer!.  clear.
+old_go_lower; entailer!.  clear.
 generalize dependent R. 
 induction n; destruct R; simpl; cancel. apply Freezer.FRZ1.
 Qed.
@@ -101,7 +101,7 @@ Lemma freeze_SEP':
  @semax cs Espec Delta (PROPx P (LOCALx Q (SEPx R))) c Post.
 Proof.
 intros. subst.
-eapply semax_pre_post. 3: eassumption. 2: intros; entailer.
+eapply semax_pre_post. 3: eassumption. 2: intros; old_go_lower; entailer.
 apply andp_left2. unfold PROPx. normalize.
 unfold LOCALx. apply derives_refl'. 
 f_equal. unfold SEPx. rewrite FRZL_ax. clear - H.
