progs/verif_reverse.v
@@ -208,12 +208,12 @@ entailer!.  (* smt_test verif_reverse_example2 *)
    unfold lseg_cons.
    apply andp_right.
    + apply prop_right.
-      destruct w_; try contradiction; intro Hx; inv Hx.
+      destruct v; try contradiction; intro Hx; inv Hx.
    + Exists h cts1 w.
       entailer!.
 * (* after the loop *)
 forward.  (* return w; *)
-Exists w_; entailer!.
+Exists w; entailer!.
 rewrite <- app_nil_end, rev_involutive.
 auto.
 Qed.
@@ -226,8 +226,9 @@ Qed.
  **)
 
 Lemma setup_globals:
- forall x,
-  (PROP  ()
+ forall Delta x,
+  (glob_types Delta) ! _three = Some (tarray t_struct_list 3) ->
+  ENTAIL Delta, PROP  ()
    LOCAL  (gvar _three x)
    SEP 
    (mapsto Ews tuint (offset_val (Int.repr 0) x) (Vint (Int.repr 1));
@@ -237,18 +238,18 @@ Lemma setup_globals:
    mapsto Ews (tptr t_struct_list) (offset_val (Int.repr 12) x)
        (offset_val (Int.repr 16) x);
    mapsto Ews tuint (offset_val (Int.repr 16) x) (Vint (Int.repr 3));
-   mapsto Ews tuint (offset_val (Int.repr 20) x) (Vint (Int.repr 0))))
+   mapsto Ews tuint (offset_val (Int.repr 20) x) (Vint (Int.repr 0)))
   |-- PROP() LOCAL(gvar _three x) 
         SEP (lseg LS Ews (map Vint (Int.repr 1 :: Int.repr 2 :: Int.repr 3 :: nil))
                   x nullval).
 Proof.
-  intros.
-  go_lower. ent_iter. rewrite prop_true_andp by auto.
+ intros.
+  go_lower.
+  rewrite !prop_true_andp by auto.
+  rewrite <- (sepcon_emp (mapsto _ _ (offset_val (Int.repr 20) _) _)).
   assert (FC: field_compatible (tarray t_struct_list 3) [] x)
-    by (apply (gvar_field_compatible _ _ _ _ H); simpl; try reflexivity; omega).
-  rewrite !sepcon_assoc.
+    by (hnf; repeat apply conj; auto; compute; auto).
   match goal with |- ?A |-- _ => set (a:=A) end.
-  rewrite sepcon_emp.
   replace x with (offset_val (Int.repr 0) x) by normalize.
   subst a.
 repeat match goal with |- _ * (mapsto _ _ _ ?q * _) |-- lseg _ _ _ (offset_val (Int.repr ?n) _) _ =>
@@ -278,7 +279,7 @@ start_function.
      (Tstruct 8%positive {| attr_volatile := false; attr_alignas := None |})
      noattr) with (tptr t_struct_list).
 eapply semax_pre; [
-  eapply derives_trans; [ | apply (setup_globals three) ] | ].
+  eapply ENTAIL_trans; [ | apply (setup_globals Delta three); auto ] | ].
  entailer!.
 forward_call (*  r = reverse(three); *)
   (Ews, map Vint [Int.repr 1; Int.repr 2; Int.repr 3], three).
